WIP: use finite map for type valuation
as with the term valuation, it is perhaps nicer to be explicit about the
domain of the variables the semantics is dealing with: in particular,
when we want to get the semantics of a term that should have no type
variables, it's nice to pass FEMPTY rather than a junky total function.
it may also be very helpful in making the correct precise statement when
it comes to doing the semantics of type and term substitution..

have changed the definition and started updating the proofs. commented
out most of the file since this breaks a lot of stuff early on.

hol-light/sholSemanticsScript.sml
@@ -152,7 +152,7 @@ val ACONV_welltyped = store_thm("ACONV_welltyped",
   metis_tac[RACONV_welltyped,EVERY_DEF])
 
 val (semantics_rules,semantics_ind,semantics_cases) = xHol_reln"semantics"`
-  (typeset τ (Tyvar s) (τ s)) ∧
+  (FLOOKUP τ s = SOME m ⇒ typeset τ (Tyvar s) m) ∧
 
   (typeset τ (Tyapp (Typrim "bool" 0) []) boolset) ∧
 
@@ -162,7 +162,7 @@ val (semantics_rules,semantics_ind,semantics_cases) = xHol_reln"semantics"`
 
   (LENGTH (tvars p) = LENGTH args ∧
    tyin = ZIP (args, MAP Tyvar (STRING_SORT (tvars p))) ∧
-   semantics FEMPTY τ (INST tyin p) mp ∧ w <: mrty ∧ holds mp w ∧
+   semantics FEMPTY FEMPTY (INST tyin p) mp ∧ w <: mrty ∧ holds mp w ∧
    INST tyin p has_type Fun rty Bool ∧ typeset τ rty mrty
    ⇒
    typeset τ (Tyapp (Tydefined op p) args) (mrty suchthat holds mp)) ∧
@@ -187,7 +187,7 @@ val (semantics_rules,semantics_ind,semantics_cases) = xHol_reln"semantics"`
   (welltyped t ∧ closed t ∧
    set(tvars t) ⊆ set (tyvars (typeof t)) ∧
    INST tyin t has_type ty ∧
-   semantics FEMPTY τ (INST tyin t) mt
+   semantics FEMPTY FEMPTY (INST tyin t) mt
    ⇒
    semantics σ τ (Const s ty (Defined t)) mt) ∧
 
@@ -201,7 +201,7 @@ val (semantics_rules,semantics_ind,semantics_cases) = xHol_reln"semantics"`
   (typeset τ (Tyapp (Tydefined op p) args) maty ∧
    tyin = ZIP(args, MAP Tyvar (STRING_SORT (tvars p))) ∧
    INST tyin p has_type Fun rty Bool ∧ typeset τ rty mrty ∧
-   semantics FEMPTY τ (INST tyin p) mp
+   semantics FEMPTY FEMPTY (INST tyin p) mp
    ⇒
    semantics σ τ (Const s (Fun rty (Tyapp (Tydefined op p) args)) (Tyabs op p))
     (abstract mrty maty (λx. if holds mp x then x else ch maty))) ∧
@@ -225,12 +225,11 @@ val typeset_Bool = store_thm("typeset_Bool",
 val _ = export_rewrites["typeset_Bool"]
 
 val type_valuation_def = Define`
-  type_valuation τ ⇔ ∀x. ∃y. y <: τ x`
+  type_valuation τ ⇔ ∀x. x ∈ FRANGE τ ⇒ ∃y. y <: x`
 
-val a_type_valuation_exists = store_thm("a_type_valuation_exists",
-  ``∃τ:string->V. type_valuation τ``,
-  rw[type_valuation_def,GSYM SKOLEM_THM] >>
-  metis_tac[BOOLEAN_IN_BOOLSET])
+val type_valuation_FEMPTY = store_thm("type_valuation_FEMPTY",
+  ``type_valuation FEMPTY``, rw[type_valuation_def])
+val _ = export_rewrites["type_valuation_FEMPTY"]
 
 val term_valuation_def = Define`
   term_valuation τ σ ⇔
@@ -261,7 +260,9 @@ val typeset_inhabited = store_thm("typeset_inhabited",
   ho_match_mp_tac type_ind >>
   conj_tac >- (
     simp[type_valuation_def] >>
-    simp[Once semantics_cases] ) >>
+    simp[Once semantics_cases] >>
+    simp[FLOOKUP_DEF,FRANGE_DEF] >>
+    metis_tac[]) >>
   rpt gen_tac >> strip_tac >>
   simp[Once semantics_cases] >>
   rw[] >- metis_tac[BOOLEAN_IN_BOOLSET]
@@ -336,6 +337,26 @@ val semantics_11 = store_thm("semantics_11",
   conj_tac >- metis_tac[typeset_inhabited] >>
   fs[] >> res_tac >> fs[])
 
+(*
+val typeset_tyvars = store_thm("typeset_tyvars",
+  ``∀ty τ1 τ2 m. typeset τ1 ty m ∧ (∀x. x ∈ set(tyvars ty) ⇒ FLOOKUP τ1 x = FLOOKUP τ2 x) ⇒ typeset τ2 ty m``,
+  ho_match_mp_tac type_ind >>
+  conj_tac >- (
+    ntac 2 (simp[Once semantics_cases]) >>
+    simp[FLOOKUP_DEF,SUBMAP_DEF,tyvars_def] >>
+    rw[]) >>
+  rpt gen_tac >> strip_tac >>
+  simp[Once semantics_cases] >> rw[] >>
+  simp[Once semantics_cases] >>
+  fs[tyvars_def,MEM_LIST_UNION] >- metis_tac[] >>
+  map_every qexists_tac[`mp`,`mrty`,`rty`,`w`] >> simp[] >>
+  fs[EVERY_MEM] >>
+  qmatch_assum_abbrev_tac`INST tyin p has_type Fun rty Bool` >>
+  qspecl_then[`sizeof p`,`p`,`
+
+  INST_CORE_HAS_TYPE
+  metis_tac[]
+
 val semantics_typeset = store_thm("semantics_typeset",
   ``(∀τ ty mty. typeset τ ty mty ⇒ type_valuation τ ⇒ ∃mt. mt <: mty) ∧
     (∀σ τ t mt. semantics σ τ t mt ⇒
@@ -343,7 +364,10 @@ val semantics_typeset = store_thm("semantics_typeset",
            ∃mty. welltyped t ∧ typeset τ (typeof t) mty ∧ mt <: mty)``,
   ho_match_mp_tac (theorem"semantics_strongind") >>
   simp[INDSET_INHABITED,FUNSPACE_INHABITED] >>
-  conj_tac >- simp[type_valuation_def] >>
+  conj_tac >- (
+    simp[type_valuation_def] >>
+    simp[FLOOKUP_DEF,FRANGE_DEF] >>
+    metis_tac[] ) >>
   conj_tac >- metis_tac[BOOLEAN_IN_BOOLSET] >>
   conj_tac >- ( rw[suchthat_def] >> metis_tac[] ) >>
   conj_tac >- (
@@ -1358,5 +1382,6 @@ val semantics_VSUBST = store_thm("semantics_VSUBST",
         metis_tac[semantics_extend_term_valuation
      *)
    cheat)
+*)
 
 val _ = export_theory()
